\section{Задача}

\begin{equation*}
  R \left( f \right)
  = \sum\limits_{t \in T} \sum\limits_{x \in X}
    \mathbb{P} \left( x,  f\left( t \right) \right)
    \cdot \mathbbm{1} \left( x = f\left( t \right) \right)
\end{equation*}

\begin{equation*}
  f^*
  = \argmin_x R \left( q \right)
  \Longrightarrow
  f^* \left( t_0 \right)
  = \argmax_x \mathbb{P} \left( x \mid  t_0 \right)
\end{equation*}

\begin{equation*}
  \mathbb{P}\left( x \mid t \right)
  = \prod_{i \in I}
    \frac{\exp{\left\{- \frac{\left( t_i - f_i\left( t \right) \right)^2}
         {2 \cdot \sigma^2} \right\}}}{\sqrt{2 \cdot \pi \cdot \sigma^2}}
  \to \max
\end{equation*}

\section{Розв'язок}

\begin{equation*}
  \ln{\mathbb{P}\left( x \mid t \right)}
  = \sum_{i \in I}
    \left\{
      - \frac{\left( t_i - f_i\left( t \right) \right)^2}{2 \cdot \sigma^2}
      - \frac{\ln{2} + \ln{\pi} + 2 \cdot \ln{\sigma}}{2}
    \right\}
  \to \max
\end{equation*}

\begin{equation*}
  \sum_{i \in I} \left( t_i - f_i\left( t \right) \right)^2 \to \min
\end{equation*}

\begin{equation*}
  \sum_{i \in I} \left( t_i - f_i\left( t \right) \right)^2
  = \sum_{i \in F} \left( t_i - f_i\left( t \right) \right)^2
  + \sum_{i \in I \setminus F} \left( t_i - f_i\left( t \right) \right)^2
\end{equation*}

\begin{equation*}
    \overline{\sigma_F^2}
    = \frac{\sum\limits_{i \in F} \left( t_i - f_i\left( t \right) \right)^2}
           {\left| F - 1 \right|}
    \Rightarrow
    \overline{\sigma_F^2}
    \sim \frac{\sum\limits_{i \in I}
                 \left( t_i - f_i\left( t \right) \right)^2}
               {\left| I \right| - 1}
\end{equation*}

\begin{equation*}
  \sum_{i \in I} \left( t_i - f_i\left( t \right) \right)^2
  \sim \left( \left| I \right| - 1 \right) \cdot \overline{\sigma_F^2}
  \to \min
\end{equation*}

\begin{equation*}
  \overline{\sigma_F^2}
  = \frac{\sum\limits_{i \in F} \left( t_i - f_i\left( t \right) \right)^2}
         {\left| F - 1 \right|}
  \to \min
\end{equation*}
