\section{Задача}

\begin{equation*}
  R \left( f \right)
  = \sum\limits_{t \in T} \sum\limits_{x \in X}
    \mathbb{P} \left( x,  f\left( t \right) \right)
    \cdot W \left( x, f\left( t \right) \right)
\end{equation*}

\begin{equation*}
  f^* = \argmin_x R \left( f \right)
\end{equation*}

\begin{equation*}
  \mathbb{P}\left( x \mid t \right)
  = \prod_{i \in I}
    \frac{\exp{\left\{- \frac{\left( t_i - f_i\left( t \right) \right)^2}
         {2 \cdot \sigma^2} \right\}}}{\sqrt{2 \cdot \pi \cdot \sigma^2}}
\end{equation*}

\subsection{Bin}

\begin{equation*}
  W \left( x, x' \right)
  = \mathbbm{1} \left( x = x' \right)
\end{equation*}

\begin{equation*}
  f^* \left( t_0 \right)
  = \argmax_x \mathbb{P} \left( x \mid  t_0 \right)
\end{equation*}

\subsection{Parameters difference}

\begin{equation*}
  W \left( x, x' \right)
  = \left\| x - x' \right\|
  = \sum_{i \in I} \left( x_i - x'_i \right)^2
\end{equation*}

\begin{equation*}
  f^* \left( t_0 \right)
  = \sum_{x \in X} x \cdot \mathbb{P}\left( x \mid t\right)
\end{equation*}

\subsection{Models difference}

\begin{equation*}
  M_v\left( k \right) = \sum_{p \in P} \alpha_p^v \cdot k_p, \qquad v \in V
\end{equation*}

\begin{equation*}
    \begin{split}
      W \left( x, x' \right)
      = \left\| M\left( x \right) - M\left( x' \right) \right\|
      = \sum_{v \in V} \left\{
          M_v\left( x \right) - M_v\left( x' \right)
        \right\}^2 = \\
      = \sum_{v \in V} \sum_{p \in P} \left\{
          \alpha_p^v \cdot \left( x_p - x'_p \right)
        \right\}^2
      = \sum_{p \in P} \left\{ \left( x_p - x'_p \right)^2
        \cdot \sum_{v \in V} \left( \alpha_p^v \right)^2 \right\} = \\
      = \left| \beta_p^2 = \sum_{v \in V} \left( \alpha_p^v \right)^2 \right|
      = \sum_{p \in P}
          \beta_p^2 \cdot \left( x_p - x'_p \right)^2
    \end{split}
\end{equation*}

\begin{equation*}
  f^* \left( t_0 \right)
  = M^-1 \left(
      \sum_{x \in X} M\left( x \right) \cdot \mathbb{P}\left( x \mid t\right)
    \right)
\end{equation*}
